Update Symbolic_Regular_Algebra_Model.thy

Symbolic_Regular_Algebra_Model.thy
@@ -34,7 +34,7 @@ subsection \<open>Regular Languages\<close>
 datatype 'a rexp =
   Zero
 | One
-| Sym "('a \<Rightarrow> bool)"
+| Atom 'a
 | Plus "'a rexp" "'a rexp"
 | Times "'a rexp" "'a rexp"
 | Star "'a rexp"
@@ -47,7 +47,7 @@ adapted from there.\<close>
 fun lang :: "'a rexp \<Rightarrow> 'a lan" where
   "lang Zero = 0"  \<comment> \<open>{}\<close>
 | "lang One = 1"  \<comment> \<open>{[]}\<close>
-| "lang (Sym f) = {[a]| a. f a}"
+| "lang (Atom a) = {[a]}"
 | "lang (Plus x y) = lang x + lang y"
 | "lang (Times x y) = lang x \<cdot> lang y"
 | "lang (Star x) = (lang x)\<^sup>\<star>" 
@@ -146,6 +146,21 @@ begin
 
 end  (* instantiation *)
 
+
+context ex_kleene_algebra begin
+
+lemma "lang (Atom (2::nat)) \<^bsup>& (lang (Atom 4) + lang (Atom 5)) = lang (Atom 2) \<^bsup>& lang (Atom 4) + lang (Atom 2) \<^bsup>& lang (Atom 5)"
+  apply simp 
+  done
+
+end
+
+lemma "(x :: 'a reg_lan) \<^bsup>& (y + z) = x \<^bsup>& y + x \<^bsup>& z"
+  by auto
+
+lemma "(x :: 'a reg_lan) \<^bsup>& (y + z) = x \<^bsup>& y + x \<^bsup>& y" 
+  nitpick
+  oops
 
 subsection \<open>Language Model of Antimirow Algebra\<close>
 
@@ -340,48 +355,38 @@ proof -
 qed
 
 
-instantiation set :: (monoid_mult) antimirow_base 
-begin
 
-definition alp_set: "\<bbbP> = {{}}"
-
-instance proof
-  fix a b c::"'a set"
-  show "(1 + a)\<^sup>\<star> = a\<^sup>\<star>" 
-    by simp
-  show "(1 \<^bsup>& a \<noteq> 0) = (\<exists>y. a = 1 + y \<and> 1 \<^bsup>& y = 0)"
-    apply(simp add: one_set_def inter_set_def c_prod_def one_list_def times_list_def)
-    by (smt (z3) Collect_empty_eq Set.set_insert Un_insert_right add.right_neutral insertCI join.sup_aci(1) plus_set_def zero_set_def)
-  show "1 \<^bsup>& (a \<cdot> b) = 1 \<^bsup>& a \<^bsup>& b"
-    sorry
-  show "1 \<^bsup>& a\<^sup>\<star> = 1"
-    apply(simp add:one_set_def inter_set_def star_def)
-    by (metis (mono_tags, lifting) Collect_cong one_set_def power_class.power.power_0 singletonI singleton_conv)
-  show "0 \<^bsup>& a = 0"
-    by simp
-next
-  fix a b :: "'a set"    
-  show "\<forall>x\<in>\<bbbP>. \<forall>y\<in>\<bbbP>. x \<cdot> a \<^bsup>& (y \<cdot> b) = x \<^bsup>& y \<cdot> (a \<^bsup>& b)"
-    by (metis (mono_tags, opaque_lifting) ab_near_semiring_one_zerol_class.annil alp_set inter_zeror singletonD zero_set_def)
-  show "\<forall>x\<in>\<bbbP>. \<forall>y\<in>\<bbbP>. a \<cdot> x \<^bsup>& (b \<cdot> y) = a \<^bsup>& b \<cdot> (x \<^bsup>& y)"
-    by (metis (mono_tags, opaque_lifting) Symbolic_Regular_Algebra_Model.alp_set ab_near_semiring_one_zero_class.annir inter_zeror singletonD zero_set_def)
-  show "\<forall>x\<in>\<bbbP>. (1::'a set) \<^bsup>& x = 0" 
-    by (metis (mono_tags, opaque_lifting) alp_set inter_zeror singletonD zero_set_def)
-qed
-
-
-interpretation lan_antimirow_l: Al_algebra "(+)" "(\<cdot>)" "1 :: 'a lan" "0"  "(\<subseteq>)" "(\<subset>)" "star" "(\<^bsup>&)" "alp"
+interpretation lan_antimirow_l: Al_algebra "(+)" "(\<cdot>)" "1 :: 'a lan" "0"  "(\<subseteq>)" "(\<subset>)" "star" "(\<^bsup>&)" "{}"
 proof
   fix x y z:: "'a lan"
   show "1 + x \<cdot> x\<^sup>\<star> = x\<^sup>\<star>"
     by simp
   show "1 \<^bsup>& y = 0 \<Longrightarrow> x = y \<cdot> x + z \<Longrightarrow> x = y\<^sup>\<star> \<cdot> z"
     using arden_l inter_empty by blast
+  show "(1 + x)\<^sup>\<star> = x\<^sup>\<star>"
+    by simp
+  show "(1 \<^bsup>& x \<noteq> 0) = (\<exists>y. x = 1 + y \<and> 1 \<^bsup>& y = 0)"
+    apply(simp add: one_set_def one_list_def inter_set_def zero_set_def plus_set_def)
+    by (meson Set.set_insert insertCI)
+  show "1 \<^bsup>& (x \<cdot> y) = 1 \<^bsup>& x \<^bsup>& y"
+    apply(simp add: one_set_def one_list_def inter_set_def zero_set_def plus_set_def)
+    by (metis Collect_cong append_is_Nil_conv l_prod_elim)
+  show "1 \<^bsup>& x\<^sup>\<star> = 1"
+    apply(simp add: one_set_def one_list_def inter_set_def zero_set_def plus_set_def)
+    by (metis (full_types) Collect_conv_if insert_subset kleene_algebra_class.dual.star_plus_one one_list_def one_set_def plus_ord_class.less_eq_def)
+  show "\<forall>x\<in>{}. 1 \<^bsup>& x = 0"
+    by (simp add: Collect_empty_eq inter_set_def one_list_def one_set_def zero_set_def)
+  show "0 \<^bsup>& x = 0"
+    by simp
+  show "\<forall>a\<in>{}. \<forall>b\<in>{}. a \<cdot> x \<^bsup>& (b \<cdot> y) = a \<^bsup>& b \<cdot> (x \<^bsup>& y)"
+    by(simp add: one_set_def one_list_def inter_set_def zero_set_def plus_set_def c_prod_def)
+  show "\<forall>a\<in>{}. \<forall>b\<in>{}. x \<cdot> a \<^bsup>& (y \<cdot> b) = x \<^bsup>& y \<cdot> (a \<^bsup>& b)"
+    by(simp add: one_set_def one_list_def inter_set_def zero_set_def plus_set_def c_prod_def)
 qed
 
-interpretation lan_antimirow_r: Ar_algebra "(+)" "(\<cdot>)" "1 :: nat lan" "0"  "(\<subseteq>)" "(\<subset>)" "star" "(\<^bsup>&)" "alp"
+interpretation lan_antimirow_r: Ar_algebra "(+)" "(\<cdot>)" "1 :: 'a lan" "0"  "(\<subseteq>)" "(\<subset>)" "star" "(\<^bsup>&)" "{}"
 proof
-  fix x y z :: "nat lan"
+  fix x y z :: "'a lan"
   show "1 + x\<^sup>\<star> \<cdot> x = x\<^sup>\<star>"
     by (metis kleene_algebra_class.star_unfoldr_eq)
   show "1 \<^bsup>& y = 0 \<Longrightarrow> x = x \<cdot> y + z \<Longrightarrow> x = z \<cdot> y\<^sup>\<star>"
@@ -389,10 +394,18 @@ proof
 qed
 
 
+context Ar_algebra begin
+
+lemma "\<forall>a\<in>{{[3]}}. \<forall>b\<in>{{[3]}}. lang (Atom (2::nat)) \<cdot> a \<^bsup>& (lang (Atom (2::nat)) \<cdot> b) = lang (Atom (2::nat)) \<^bsup>& lang (Atom (2::nat)) \<cdot> (a \<^bsup>& b)"
+  apply simp 
+  done
+end
+
+
 subsection \<open>Regular Language Model of Antimirow Algebra\<close>
 
 notation
-  Sym ("\<langle>_\<rangle>") and
+  Atom ("\<langle>_\<rangle>") and
   Plus (infixl "+\<^sub>r" 65) and
   Times (infixl "\<cdot>\<^sub>r" 70) and
   Inter (infixl "&\<^sub>r" 70) and
@@ -532,13 +545,12 @@ next
       by (metis assms lang.simps(6) r1(1) r2 r_lang.abs_eq r_lang.rep_eq)
   qed
 qed
-end
     
-instantiation reg_lan :: (monoid_mult) Ar_algebra
+instantiation reg_lan :: (type) Ar_algebra
 begin
 
-definition alp_reg_lan::"'a Symbolic_Regular_Algebra_Model.reg_lan set" where
-  "alp_reg_lan = {}"
+definition alp_reg_lan :: "'a reg_lan set" where 
+"alp_reg_lan = {}"
 
 instance proof
   fix x :: "'a reg_lan"
@@ -551,11 +563,11 @@ next
 next
   fix x y z :: "'a reg_lan"
   show "1 \<^bsup>& (x \<cdot> y) = 1 \<^bsup>& x \<^bsup>& y"
-    by (metis A13 Symbolic_Regular_Algebra_Model.one_reg_lan.rep_eq Symbolic_Regular_Algebra_Model.reg_lan.Rep_reg_lan_inject Symbolic_Regular_Algebra_Model.times_reg_lan.rep_eq inter_reg_lan.rep_eq)
+    by (metis Symbolic_Regular_Algebra_Model.one_reg_lan.rep_eq Symbolic_Regular_Algebra_Model.reg_lan.Rep_reg_lan_inject Symbolic_Regular_Algebra_Model.times_reg_lan.rep_eq inter_reg_lan.rep_eq lan_antimirow_l.A13)
 next 
   fix x :: "'a reg_lan"
   show "1 \<^bsup>& x\<^sup>\<star> = 1"
-    by (metis A14 Symbolic_Regular_Algebra_Model.one_reg_lan.rep_eq Symbolic_Regular_Algebra_Model.reg_lan.Rep_reg_lan_inject Symbolic_Regular_Algebra_Model.star_reg_lan.rep_eq inter_reg_lan.rep_eq)
+    by (metis Symbolic_Regular_Algebra_Model.one_reg_lan.rep_eq Symbolic_Regular_Algebra_Model.reg_lan.Rep_reg_lan_inject Symbolic_Regular_Algebra_Model.star_reg_lan.rep_eq inter_reg_lan.rep_eq lan_antimirow_l.dual.A14)
 next 
   fix x y z :: "'a reg_lan"
   show "1 \<^bsup>& y = 0 \<Longrightarrow> x = x \<cdot> y + z \<Longrightarrow> x = z \<cdot> y\<^sup>\<star>"
@@ -576,12 +588,12 @@ next
       apply (transfer, auto)
       using zero_set_def apply auto[1]
         apply (simp add: zero_set_def)
-        subgoal 
-          by (smt (verit, ccfv_threshold) Symbolic_Regular_Algebra_Model.lang.simps(2) Symbolic_Regular_Algebra_Model.lang.simps(4) Symbolic_Regular_Algebra_Model.rexp.distinct(1) antimirow_base_class.EWP empty_iff join.sup_left_idem rexp_ewp.simps(2) rexp_ewp.simps(4) rexp_ewp_l_ewp zero_set_def)
+      subgoal 
+        by (metis (mono_tags, lifting) Symbolic_Regular_Algebra_Model.lang.simps(2) Symbolic_Regular_Algebra_Model.rexp.simps(7) empty_iff join.sup_left_idem l_ewp_def lan_antimirow_l.dual.EWP one_list_def one_set_def plus_ord_class.less_eq_def rexp_ewp_l_ewp zero_set_def)
         subgoal 
           using zero_set_def by auto
         subgoal 
-          by (metis antimirow_base_class.EWP)
+          by (metis lan_antimirow_l.dual.EWP)
         done
   qed
 next 
@@ -598,7 +610,7 @@ next
 qed
 end
 
-instantiation reg_lan :: (monoid_mult) Al_algebra
+instantiation reg_lan :: (type) Al_algebra
 begin
 
 instance proof
@@ -612,7 +624,7 @@ next
 qed
 end
 
-instance reg_lan :: (monoid_mult) A_algebra ..
+instance reg_lan :: (type) A_algebra ..
 
 theorem arden_regexp_l: 
   assumes "ro(y) = 0\<^sub>r" "x \<sim> y \<cdot>\<^sub>r x +\<^sub>r z" 
@@ -626,9 +638,5 @@ theorem arden_regexp_r:
   using assms
   by (metis Symbolic_Regular_Algebra_Model.lang.simps(4) Symbolic_Regular_Algebra_Model.lang.simps(5) Symbolic_Regular_Algebra_Model.lang.simps(6) Symbolic_Regular_Algebra_Model.rexp.simps(7) arden_r r_lang.abs_eq r_lang.rep_eq rexp_ewp_l_ewp)
 
-context A_algebra begin
-
-
-end
 
 end
